erasure/theories/ESubstitution.v
@@ -108,17 +108,17 @@ Proof.
   all: try now (econstructor; eauto).
   all: try now (econstructor; eapply Is_type_extends; eauto).
   - econstructor. all:eauto.
-    2:{ eauto. eapply All2_All_left in X3.
+    2:{ eauto. eapply All2_All_left in X4.
         2:{ intros ? ? []. exact e. }
-        eapply All2_All_mix_left in X3; eauto.
-        eapply All2_impl. exact X3.
+        eapply All2_All_mix_left in X4; eauto.
+        eapply All2_impl. exact X4.
         intros. destruct H as [? []].
         split; eauto. }
     eapply Computational_extends; eauto.
   - econstructor. all:eauto.
     eapply SingletonProp_extends; eauto.
     eapply Is_type_extends; eauto.
-    inv X3. eapply X7; eauto.
+    inv X4. eapply X8; eauto.
   - eapply erases_tCase_Empty; eauto.
     eapply SingletonProp_extends; eauto.
   - econstructor. destruct isdecl. 2:eauto.
@@ -207,7 +207,7 @@ Proof.
     + eauto.
     + eapply h_forall_Γ0; eauto.
     + eapply All2_map.
-      eapply All2_All_left in X3.
+      eapply All2_All_left in X4.
       2:{ intros ? ? [? e]. exact e. }
       eapply All2_impl. eapply All2_All_mix_left.
       eassumption. eassumption. intros.
@@ -400,19 +400,19 @@ Proof.
     + cbn. econstructor.
     + econstructor.
       eapply is_type_subst; eauto.
-  - depelim H5.
+  - depelim H4.
     + cbn. econstructor.
       * eauto.
-      * eapply H4; eauto.
+      * eapply H3; eauto.
       * eapply All2_map.
         eapply All2_impl_In; eauto.
-        intros. destruct H11, x, y. cbn in *. subst. split; eauto.
-        eapply All2_All_left in X3.
+        intros. destruct H10, x, y. cbn in *. subst. split; eauto.
+        eapply All2_All_left in X4.
         2:{ intros ? ? []. exact e0. }
 
-        eapply In_nth_error in H9 as [].
-        eapply nth_error_all in X3; eauto.
-        eapply X3; eauto.
+        eapply In_nth_error in H8 as [].
+        eapply nth_error_all in X4; eauto.
+        eapply X4; eauto.
     (* + cbn. econstructor. *)
     (*   eapply H4 in H5; eauto. *)
     (*   econstructor. *)
