pcuic/theories/PCUICWeakening.v
@@ -556,7 +556,7 @@ Qed.
 Lemma lift_types_of_case ind mdecl idecl args u p pty indctx pctx ps btys n k :
   let f k' := lift n (k' + k) in
   let f_ctx := lift_context n k in
-  closed_ctx mdecl.(ind_params) ->
+  closed_ctx (subst_instance_context u (ind_params mdecl)) ->
   types_of_case ind mdecl idecl args u p pty = Some (indctx, pctx, ps, btys) ->
   types_of_case ind mdecl (map_one_inductive_body (context_assumptions mdecl.(ind_params))
                                                   (length (arities_context mdecl.(ind_bodies)))
@@ -567,9 +567,10 @@ Proof.
   simpl. intros closedpars.
   unfold types_of_case.
   rewrite -> ind_type_map. simpl.
-  pose proof (lift_instantiate_params n k (ind_params mdecl) args (ind_type idecl)) as H.
-  erewrite <- H ; trivial. clear H.
-  case_eq (instantiate_params (ind_params mdecl) args (ind_type idecl)) ; try discriminate.
+  epose proof (lift_instantiate_params n k _ args (subst_instance_constr u (ind_type idecl))) as H.
+  rewrite <- lift_subst_instance_constr.
+  erewrite <- H; trivial. clear H.
+  case_eq (instantiate_params (subst_instance_context u (ind_params mdecl)) args (subst_instance_constr u (ind_type idecl))) ; try discriminate.
   intros ity eq. simpl.
   pose proof (lift_destArity [] ity n k); trivial. simpl in H.
   unfold lift_context, fold_context in H. simpl in H. simpl. rewrite -> H. clear H.
@@ -745,11 +746,11 @@ Proof.
   unfold check_correct_arity. intro H.
   inversion H; subst. simpl. rewrite lift_context_snoc0.
   constructor.
-  - apply All2_length in H4. destruct H4.
-    clear -H2. apply (lift_eq_decl _ #|Γ''| (#|indctx| + #|Γ'|)) in H2.
-    unfold lift_decl, map_decl in H2; cbn in H2.
+  - apply All2_length in X0. destruct X0.
+    clear -X. apply (lift_eq_decl _ #|Γ''| (#|indctx| + #|Γ'|)) in X.
+    unfold lift_decl, map_decl in X; cbn in X.
     assert (XX : lift #|Γ''| (#|indctx| + #|Γ'|) (mkApps (tInd ind u) (map (lift0 #|indctx|) (firstn npar args) ++ to_extended_list indctx)) = mkApps (tInd ind u) (map (lift0 #|lift_context #|Γ''| #|Γ'| indctx|) (firstn npar (map (lift #|Γ''| #|Γ'|) args)) ++ to_extended_list (lift_context #|Γ''| #|Γ'| indctx)));
-      [|now rewrite XX in H2].
+      [|now rewrite XX in X].
 
     rewrite -> lift_mkApps, map_app.
     rewrite -> firstn_map. rewrite -> to_extended_list_lift.
@@ -855,11 +856,12 @@ Proof.
         -- destruct isdecl as [Hmdecl Hidecl].
            eapply on_declared_minductive in Hmdecl; eauto.
            eapply onParams in Hmdecl.
+           rewrite closedn_subst_instance_context.
            eapply closed_wf_local in Hmdecl; eauto. }
     -- erewrite -> lift_declared_inductive; eauto.
     -- auto.
     -- auto.
-    -- revert H1.
+    -- revert X2.
        subst pars.
        erewrite lift_declared_inductive; eauto.
        apply lift_check_correct_arity.
